a first proof for the checker

ifc/extended/Testing/SSNI.v
@@ -17,71 +17,83 @@ Open Scope string_scope.
 Require Import Show.
 
 Require Import Reachability.
-Definition propSSNI_helper (t : table) (v : Variation) : Property :=
-  let '(Var lab st1 st2) := v in
-(*  Property.trace (Show.show lab ++ Show.nl ++
-     showStatePair lab frameMap1 frameMap2 st1 st2) *)
 
-  collect (option_bind opcode_of_instr
-            (instr_lookup (st_imem st1) (st_pc st1))) 
 
-(* collect (show lab) *)
-  (let is_low_state st := isLow (pc_lab (st_pc st)) lab in
-  if indist lab st1 st2 then
-     (* XXX Our generator should always give us this by design.
-            If that's not the case the generator is broken. *)
-     match exec t st1 with
-       | Some (tr1, st1') =>
-         if is_low_state st1 then
-           match exec t st2 with
-             | Some (tr2, st2') =>
-               collect "LOW -> *" (
-               whenFail ("LOW -> *" ++ nl ++
-                        (show_execution lab [st1; st1'] [st2; st2']))
-                   (observe_comp (observe lab tr1) (observe lab tr2) 
-                    && (indist lab st1' st2'))
-               )
-             | _ => (* 1 took a low step and 2 failed *)
-               collect "Second failed" (property true)
-(*
+Section Checkers.
+  Context {Gen : Type -> Type}
+          {H : GenMonad Gen}.
+  
+  Definition Property := Property Gen.
+
+
+  Definition is_low_state st lab := isLow (pc_lab (st_pc st)) lab.
+
+
+  Definition propSSNI_helper (t : table) (v : Variation) : Property :=
+    let '(Var lab st1 st2) := v in
+    (*  Property.trace (Show.show lab ++ Show.nl ++
+     showStatePair lab frameMap1 frameMap2 st1 st2) *)   
+    collect (option_bind opcode_of_instr
+                         (instr_lookup (st_imem st1) (st_pc st1))) 
+            
+    (* collect (show lab) *)
+            (if indist lab st1 st2 then
+               (* XXX Our generator should always give us this by design.
+                  If that's not the case the generator is broken. *)
+               match exec t st1 return Property with
+                 | Some (tr1, st1') =>
+                   if is_low_state st1 lab then
+                     match exec t st2 with
+                       | Some (tr2, st2') =>
+                         collect "LOW -> *" (
+                                   whenFail 
+                                     ("LOW -> *" ++ nl ++
+                                                 (show_execution lab [st1; st1'] [st2; st2']))
+                                     (observe_comp (observe lab tr1) (observe lab tr2) 
+                                                   && (indist lab st1' st2')))
+                       | _ => (* 1 took a low step and 2 failed *)
+                         collect "Second failed" (property true)
+                     (* 
                 ((Property.trace (show_pair lab st1 st1'))
                 (property false))
-*)
-               (* XXX This used to fail the property in ICFP paper.
+                      *)
+                     (* XXX This used to fail the property in ICFP paper.
                   But here it does happen for Alloc, Store and BRet *)
-           end
-         else (* is_high st1 *)
-           if is_low_state st1' then
-             match exec t st2 with
-               | Some (tr2, st2') =>
-                 if is_low_state st2' then 
-                   collect "HIGH -> LOW" (
-                   (whenFail ("HIGH -> LOW" ++ Show.nl ++
-                               (show_execution lab [st1; st1'] [st2; st2']))
-                             (observe_comp (observe lab tr1) (observe lab tr2) 
-                              && (indist lab st1' st2')))
-                   )
-                 else collect "Second not low" (property true)
-                      (* This can happen; it's just a discard *)
-                      (* TODO: could check that st2' `indist` st1 *)
-               | _ => collect "Second failed H" (property true)
-                      (* This can happen; it's just a discard *)
-             end
-           else
-             collect "HIGH -> HIGH" (
-             whenFail ("HIGH -> HIGH" ++ Show.nl ++
-                         (show_pair lab st1 st1'))
-                      (beq_nat (List.length (observe lab tr1)) 0 
-                       && indist lab st1 st1')
-             )
-       | _ => collect "Failed" (property true)
-              (* This can happen; it's just a discard *)
-              (* TODO: could check if st2 does a H -> H step *)
-     end
-  else collect "Not indist!" (property true)).
-       (* XXX this should never happen with a correct generator;
+                     end
+                   else (* is_high st1 *)
+                     if is_low_state st1' lab then
+                       match exec t st2 with
+                         | Some (tr2, st2') =>
+                           if is_low_state st2' lab then 
+                             collect "HIGH -> LOW" (
+                                       (whenFail ("HIGH -> LOW" ++ Show.nl ++
+                                                                (show_execution lab [st1; st1'] [st2; st2']))
+                                                 (observe_comp (observe lab tr1) (observe lab tr2) 
+                                                               && (indist lab st1' st2')))
+                                     )
+                           else collect "Second not low" (property true)
+                         (* This can happen; it's just a discard *)
+                         (* TODO: could check that st2' `indist` st1 *)
+                         | _ => collect "Second failed H" (property true)
+                       (* This can happen; it's just a discard *)
+                       end
+                     else
+                       collect "HIGH -> HIGH" (
+                                 whenFail ("HIGH -> HIGH" ++ Show.nl ++
+                                                          (show_pair lab st1 st1'))
+                                          (beq_nat (List.length (observe lab tr1)) 0 
+                                       && indist lab st1 st1')
+                               )
+                 | _ => collect "Failed" (property true)
+               (* This can happen; it's just a discard *)
+               (* TODO: could check if st2 does a H -> H step *)
+               end
+             else collect "Not indist!" (property true)).
+           (* XXX this should never happen with a correct generator;
               and prop_generate_indist already tests this;
               so this should either go away or become (propery false) *)
 
-Definition propSSNI t : Property := 
-  forAllShrink (fun _ => ""%string) gen_variation_state (fun _ => nil) (* shrinkVState *) (propSSNI_helper t).
+  Definition propSSNI t : Property := 
+    forAllShrink (fun _ => ""%string) gen_variation_state (fun _ => nil) (* shrinkVState *) (propSSNI_helper t).
+
+End Checkers.
