ifc/extended/Testing/SSNICheckers_Proofs.v
@@ -1,0 +1,181 @@
+Require Import String.
+Require Import Arith.EqNat.
+Require Import ZArith.
+
+Require Import Machine.
+
+Require Import QuickChick EndToEnd SetOfOutcomes.
+
+Require Import Common.
+Require Import Printing.
+Require Import Shrinking.
+Require Import Generation.
+Require Import Indist.
+Require Import SSNI. 
+
+Require Import ssreflect ssrbool eqtype.
+
+Require Import Show.
+
+(* Possible steps according to SSNI_helper*)
+
+(*
+
+L ->  s1'
+      |    final states indistinguishable
+L ->  s2'
+
+
+
+
+L ->  s1'
+      
+L ->  x    no step for the second state
+
+
+
+H -> L
+     |     final states indistinguishable
+H -> L 
+
+
+
+
+H -> L
+         no condition here. Seems a bit strange. 
+H -> H 
+
+
+
+H -> H   high to high step. Requires no trace and the states before and 
+         after to be indistinguishable
+
+*)
+
+
+Definition propSSNI_prop (t : table) (v : Variation) : Prop := 
+  let '(Var lab st1 st2) := v in
+  (indist lab st1 st2) ->
+  (is_low_state st1 lab /\ (forall tr1 st1' tr2 st2', 
+                          exec t st1 = Some (tr1, st1') ->
+                          exec t st2 = Some (tr2, st2') ->
+                          observe_comp (observe lab tr1) (observe lab tr2) /\ 
+                          (indist lab st1' st2'))) \/
+  (~~ is_low_state st1 lab /\ (forall tr1 st1', 
+                             exec t st1 = Some (tr1, st1') -> 
+                             ((is_low_state st1' lab /\
+                               forall tr2 st2',
+                                 exec t st2 = Some (tr2, st2') -> 
+                                 is_low_state st2' lab ->
+                                 observe_comp (observe lab tr1) (observe lab tr2) /\ 
+                                 (indist lab st1' st2')) \/
+                              (~~ is_low_state st1' lab /\
+                               List.length (observe lab tr1) = 0%nat /\
+                               indist lab st1 st1')))).
+
+Definition propSSNI_bool (t : table) (v : Variation) : bool :=
+    let '(Var lab st1 st2) := v in
+    if indist lab st1 st2 then
+      match exec t st1  with
+        | Some (tr1, st1') =>
+          if is_low_state st1 lab then
+            match exec t st2 with
+              | Some (tr2, st2') =>
+                (observe_comp (observe lab tr1) (observe lab tr2) 
+                              && (indist lab st1' st2'))
+              | _ => true
+            end
+          else (* is_high st1 *)
+            if is_low_state st1' lab then
+              match exec t st2 with
+                | Some (tr2, st2') =>
+                  if is_low_state st2' lab then
+                    observe_comp (observe lab tr1) (observe lab tr2) 
+                                 && (indist lab st1' st2')
+                  else true
+                | _ => true
+              end
+            else
+              beq_nat (List.length (observe lab tr1)) 0 
+                      && indist lab st1 st1'
+        | _ => true
+      end
+    else true.
+
+Lemma ssniP: 
+  forall (t : table) v,
+    reflect (propSSNI_prop t v) (propSSNI_bool t v).
+Proof. 
+  move=> t [lab st1 st2]. apply/(@iffP (propSSNI_bool t (Var lab st1 st2))); try (by apply idP);
+  rewrite /propSSNI_bool /propSSNI_prop.
+  { destruct (indist lab st1 st2) => //.
+    destruct (exec t st1) as [ [tr1' st1'] |]. 
+    - destruct (is_low_state st1 lab).    
+      + destruct (exec t st2) as [ [tr2' st2'] |];
+        move => H _; left; split => //. 
+        move=> tr1_ st1'_ st2_ st2'_ [eq1 eq2] [eq3 eq4]; subst.
+        by apply/andP.
+      + move => H _. right. split => //. 
+        move=> tr1_ st1'_ [eq1 eq2]; subst.  
+        destruct (exec t st2) as [[tr2' st2'] |].
+        * destruct (is_low_state st1'_ lab).
+          left. split => //. move => tr2_ st2'_ [eq1 eq2] H'; subst.
+          destruct (is_low_state st2'_ lab); try congruence.
+          by apply/andP.
+          right. split=> //. move : H => /andP [H1 H2]. split => //.
+          by apply beq_nat_eq.
+        * destruct (is_low_state st1'_ lab). left. by split => //.
+          right. split => //. move : H => /andP [H1 H2]. split => //.
+          by apply beq_nat_eq.
+    - move=> _ _. destruct (is_low_state st1 lab). 
+      + left. split => //.
+      + right. split => //. }
+  { destruct (indist lab st1 st2) => //. move => /(_ is_true_true) H.
+    move: H => [[H1 H2] | [H1 H2]]. 
+    - rewrite H1. destruct (exec t st1) as [ [tr1' st1'] |] => //. 
+      destruct (exec t st2) as [ [tr2' st2'] |] => //.
+      apply/andP. by auto. 
+    - apply Bool.negb_true_iff  in H1. rewrite H1. 
+      destruct (exec t st1) as [ [tr1' st1'] |] => //.
+      move : H2 => /(_ _ _ Logic.eq_refl) [[H2 H3] | [H2 [H3 H4]]].
+      + rewrite H2. destruct (exec t st2) as [ [tr2' st2'] |] => //.
+        move: H3 => /(_ _ _ Logic.eq_refl) H3.
+        destruct (is_low_state st2' lab) => //. apply/andP; by auto.
+      + apply Bool.negb_true_iff in H2. rewrite H2.
+        apply/andP. split => //. by apply beq_nat_true_iff in H3. }
+Qed.
+    
+Lemma propSSNI_helper_equiv:
+  forall (t : table) v, 
+    semProperty (@propSSNI_helper Pred _ t v) <-> propSSNI_prop t v.
+Proof. 
+  move=> t [lab st1 st2]. split; [move => H; apply/ssniP| move=> /ssniP H];
+  rewrite /propSSNI_helper /propSSNI_bool /semTestable semCollect_idemp in H *. 
+  - move=> /semPredQProp H. destruct (indist lab st1 st2) => //. 
+    { destruct (exec t st1) as [ [tr1' st1'] |] => //. 
+      destruct (is_low_state st1 lab). 
+      - destruct (exec t st2) as [ [tr2' st2'] |] => //.  
+          by move/semCollect_idemp/semPredQProp
+                 /semWhenFail_idemp/semBool : H => H. 
+      - destruct (is_low_state st1'). 
+        + destruct (exec t st2) as [[tr2 st2'] |] => //.
+          destruct (is_low_state st2' lab).
+            by move/semCollect_idemp/semPredQProp/semWhenFail_idemp/semBool : H.
+            by move/semCollect_idemp/semPredQProp/semBool : H.
+        + by move/semCollect_idemp/semPredQProp/semWhenFail_idemp/semBool : H. }
+  -  move=> H. 
+     destruct (indist lab st1 st2); try by apply/semPredQProp/semCollect_idemp/semBool.
+    { destruct (exec t st1) as [ [tr1' st1'] |]. 
+      destruct (is_low_state st1 lab).  
+      - destruct (exec t st2) as [ [tr2' st2'] |].
+        by apply/semPredQProp/semCollect_idemp/semPredQProp/semWhenFail_idemp/semBool.
+        by apply/semPredQProp/semCollect_idemp/semBool.
+      - destruct (is_low_state st1'). 
+        + destruct (exec t st2) as [[tr2 st2'] |].
+          * destruct (is_low_state st2' lab).
+            by apply/semPredQProp/semCollect_idemp/semPredQProp/semWhenFail_idemp/semBool.
+            by apply/semPredQProp/semCollect_idemp/semBool.
+          * by apply/semPredQProp/semCollect_idemp/semBool.
+        + by apply/semPredQProp/semCollect_idemp/semPredQProp/semWhenFail_idemp/semBool.
+      - by apply/semPredQProp/semCollect_idemp/semBool. }
+Qed.
